test-suite/bugs/closed/bug_11189.v
@@ -1,0 +1,10 @@
+Structure trivial_cs := { key : Type }.
+
+Canonical Structure base : trivial_cs := {|key := unit|}.
+Canonical Structure step {A : Type} (t : trivial_cs) : trivial_cs := {| key := A -> key t |}.
+
+Definition test := fun (t : trivial_cs) (k : key t) => tt.
+
+Check test (_) (fun x : unit => tt).
+
+Check (fun (x : key _) => x tt).
